Main: Add --list_plugins option

src/basic/FStar.Options.fst
@@ -268,6 +268,7 @@ let defaults =
       ("query_cache"                  , Bool false);
       ("query_stats"                  , Bool false);
       ("read_checked_file"            , Unset);
+      ("list_plugins"                 , Bool false);
       ("read_krml_file"               , Unset);
       ("record_hints"                 , Bool false);
       ("record_options"               , Bool false);
@@ -524,6 +525,7 @@ let get_query_cache             ()      = lookup_opt "query_cache"              
 let get_query_stats             ()      = lookup_opt "query_stats"              as_bool
 let get_read_checked_file       ()      = lookup_opt "read_checked_file"        (as_option as_string)
 let get_read_krml_file          ()      = lookup_opt "read_krml_file"           (as_option as_string)
+let get_list_plugins            ()      = lookup_opt "list_plugins"             as_bool
 let get_record_hints            ()      = lookup_opt "record_hints"             as_bool
 let get_record_options          ()      = lookup_opt "record_options"           as_bool
 let get_retry                   ()      = lookup_opt "retry"                    as_bool
@@ -1590,6 +1592,12 @@ let rec specs_with_types warn_unsafe : list (char & string & opt_type & Pprint.d
      WithSideEffect ((fun _ -> display_debug_keys(); exit 0),
                      (Const (Bool true))),
     text "List all debug keys and exit");
+
+  (* FIXME: all of these should really be modes, not a boolean option *)
+  ( noshort,
+    "list_plugins",
+     Const (Bool true),
+    text "List all registered plugins and exit");
   ]
 
 and specs (warn_unsafe:bool) : list (FStar.Getopt.opt & Pprint.document) =
@@ -2083,6 +2091,7 @@ let quake_keep                   () = get_quake_keep                  ()
 let query_cache                  () = get_query_cache                 ()
 let query_stats                  () = get_query_stats                 ()
 let read_checked_file            () = get_read_checked_file           ()
+let list_plugins                 () = get_list_plugins                ()
 let read_krml_file               () = get_read_krml_file              ()
 let record_hints                 () = get_record_hints                ()
 let record_options               () = get_record_options              ()
