src/basic/FStar.Options.fsti
@@ -172,6 +172,7 @@ val no_smt                      : unit    -> bool
 val normalize_pure_terms_for_extraction
                                 : unit    -> bool
 val krmloutput                  : unit    -> option string
+val list_plugins                : unit    -> bool
 val output_deps_to              : unit    -> option string
 val output_dir                  : unit    -> option string
 val prepend_cache_dir           : string  -> string
